Foundation/Propositional/Neighborhood/NB/Logic.lean
@@ -1,5 +1,0 @@
-module
-
-public import Foundation.Propositional.Neighborhood.NB.Logic.WF
-@[expose] public section
-end
